New progam_logic directory structure.

rocq-osiris/theories/program_logic/rules/handler_rules.v
@@ -1,14 +1,17 @@
 From iris.proofmode Require Import proofmode.
+From iris.base_logic.lib Require Import gen_heap.
 
 From osiris Require Import base.
 From osiris.lang Require Import lang.
 From osiris.program_logic Require Import thread_step ewp tactics.
-From osiris.program_logic.rules Require Import impure_rules stop_rules.
+From osiris.program_logic.rules Require Import basic_rules impure_rules stop_rules.
 From osiris.semantics Require Import code.
 
 From osiris.program_logic.pure Require Import pure.
 
 From Stdlib Require Import FunctionalExtensionality.
+
+Import ewp_rules_tactics.
 
 (* -------------------------------------------------------------------------- *)
 (** *Shallow and deep handlers *)
@@ -197,6 +200,182 @@ End handler_specifications.
 Ltac deep_handler_spec_unfold :=
   rewrite deep_handler_spec_unfold /deep_handler_spec_pre /=.
 
+(** * Shallow handler specification. *)
+
+ Definition shallow_handler_spec `{!osirisGS Σ} E Ψ (Q : outcome2 val exn → iProp Σ)
+    (h : code.outcome3 val exn -> microvx)
+    Ψ' Q' :=
+    ((* [Return] and [Exception] branch *)
+    (∀ o, Q o -∗ ▷ ewp_def E (h o) Ψ' Q') ∧
+
+    (* [Effect] branch *)
+    (∀ v k, Ψ allows perform v
+          << λ o, ▷ ewp_def E (stop CResume (k, o)) Ψ Q >> -∗
+        ▷ ewp_def E (h (O3Perform v k)) Ψ' Q'))%I.
+
+Section handle_rules.
+
+  Context `{!osirisGS Σ}.
+
+  Context {A X : Type}.
+  Context {E : coPset} {Ψ : iEff Σ} {Q : outcome2 A X → iProp Σ}.
+
+  Implicit Type m : micro A X.
+
+  (* Specification for [Handle] follows the specification for shallow handlers. *)
+  Lemma ewp_handle Ψ' Φ' Φ e h:
+    ewp_def E e Ψ Φ -∗
+    shallow_handler_spec E Ψ Φ h Ψ' Φ' -∗
+    ewp_def E (Handle e h) Ψ' Φ'.
+  Proof.
+    (* We proceed by Löb-induction after generalizing [e] [h] and [eh]. *)
+
+    iIntros "He Hsh".
+    iLöb as "IH" forall (e).
+    ewp_unfold_head.
+    intro_state.
+
+    ewp_mask_intro "Hmod".
+    construct_wp_nonret; destruct_thread_step; cbn; iMod "Hmod" as "_"; cbn; rename π into π'.
+
+    { (* [StepHandleRet] *)
+      ewp_unfold (@ret C.val exn v).
+      iFrame.
+      iDestruct "Hsh" as "[Hsh _]";
+      iSpecialize ("Hsh" with "He");
+      iMod "Hsh";
+      ewp_mask_intro "Hmod"; ewp_mask_elim.
+      iApply "Hsh". }
+
+    { (* [StepHandleThrow] *)
+      ewp_unfold (@throw C.val exn e0).
+      iFrame.
+      iDestruct "Hsh" as "(Hsh & _)".
+      iSpecialize ("Hsh" with "He");
+      iMod "Hsh";
+      ewp_mask_intro "Hmod"; ewp_mask_elim.
+      iApply "Hsh". }
+
+    { (* [StepHandlePerform] *)
+      iDestruct "Hsh" as "[_ Hsh]".
+      ewp_unfold (Stop CPerf e0 k).
+      iMod "He" as "HP".
+
+      iDestruct (gen_heap_alloc _ _ (K k) with "Hsi") as ">[Hsi [HH _]]";
+        [ exact H | ].
+
+      iAssert (Ψ allows perform e0
+                 << fun o => ▷ ewp_def E (stop CResume (l, o)) Ψ Φ >>)%I
+        with "[HP HH]" as "HΨ".
+      { iApply (monotonic_prot with "[HH] HP").
+        iIntros (?) "Hwp"; cbn. iNext.
+        rename σ into σ'.
+        ewp_unfold_head.
+        intro_state. ewp_mask_intro "Hmod".
+        iDestruct (gen_heap_valid with "Hsi HH") as %Hl.
+        construct_wp_nonret.
+        eapply invert_thread_step_resume in Hstep; [ | eexact Hl ].
+        destruct Hstep as (-> & -> & ->).
+        rewrite try2_inject2_right.
+        iDestruct (gen_heap_update with "Hsi HH") as ">(Hsi & HH)".
+        iFrame.
+        by ewp_mask_elim. }
+
+      iSpecialize ("Hsh" with "HΨ").
+      ewp_mask_intro "Hmod"; ewp_mask_elim.
+      iFrame. }
+
+    { (* [StepHandleFork] *)
+      ewp_mask_intro "Hmod". iModIntro. iMod "Hmod". iModIntro. iFrame.
+      destruct x.
+      ewp_unfold_all. intro_state. spec_state. iModIntro.
+      destruct Hstep as (? & ? & ? & Htstep).
+      destruct_thread_step.
+      construct_wp_nonret.
+      destruct_thread_step.
+      eassert (thread_step (σ'0, Stop CFork (v, v0) k, dom π) _) as Htstep.
+      { eapply ForkS. eassumption. }
+      spec_step.
+      ewp_mask_elim.
+      iMod "He" as "(Hwp & $)".
+      iModIntro.
+      iApply ("IH" with "Hwp Hsh"). }
+
+    { (* [StepHandleJoin] *)
+      ewp_mask_intro "Hmod". iModIntro. iMod "Hmod". iModIntro. iFrame.
+      ewp_unfold_all. intro_state. spec_state. iMod "He". iModIntro.
+      destruct (π !! ι); last done.
+      iDestruct "He" as "(%φ' & $ & He)".
+      iIntros "!> %o Ho". iSpecialize ("He" with "Ho").
+      ewp_mask_elim.
+      iMod "He" as "(He & $)". iModIntro.
+      iApply ("IH" with "He Hsh"). }
+
+    { (* [StepHandleCrash] *)
+      ewp_unfold (@Crash val exn).
+      by iMod "He". }
+
+    { (* [StepHandleLeft] *)
+      eassert (thread_step (σ, e, dom π') _) as Hstep.
+      { apply BaseS. eassumption. }
+      iCombine "Hsi Hti" as "Hsi".
+      iPoseProof (ewp_step _ _ _ Hstep with "Hsi He") as ">H".
+      iMod "H". ewp_mask_elim. iMod "H" as "(H & $)". iModIntro.
+      iApply ("IH" with "H Hsh"). }
+  Qed.
+
+  (* Inversion for [Handle] *)
+  Lemma ewp_handle_resume {B Y} k l w (c : _ -> micro B Y) Φ :
+    isCont l k -∗
+    ewp_def E (Handle (k w) c) Ψ Φ -∗
+    ewp_def E (Handle (resume l w) c) Ψ Φ.
+  Proof.
+    destruct Ψ.
+    iIntros "Hl H".
+    ewp_unfold_head; intro_state; ewp_mask_intro "Hmod".
+    construct_wp_nonret.
+
+    (* Argue that [l] must be in the domain of the ghost heap. *)
+    iDestruct (gen_heap.gen_heap_valid with "Hsi Hl")  as "%".
+
+    destruct_thread_step.
+    eapply invert_step_resume in H; [ destruct H | eauto ]; subst.
+    (* Thus, the reduction step must be a successful step. *)
+
+    (* Update the ghost heap. *)
+    iMod (gen_heap.gen_heap_update with "Hsi Hl") as "[Hsi Hl]".
+    ewp_mask_elim. iFrame.
+    by rewrite try2_inject2_right.
+  Qed.
+
+  (* Variant inversion rule for [Handle] *)
+  Lemma ewp_handle_inv' k l w (c : _ -> micro A X)  :
+    isCont l k -∗
+    ▷ (isShot l -∗
+        ewp_def E (Handle (k w) c) Ψ Q) -∗
+    ewp_def E (Handle (stop CResume (l, w)) c) Ψ Q.
+  Proof.
+    destruct Ψ.
+    iIntros "Hl H".
+    ewp_unfold_head; intro_state; ewp_mask_intro "Hmod".
+    construct_wp_nonret.
+
+    (* Argue that [l] must be in the domain of the ghost heap. *)
+    iDestruct (gen_heap.gen_heap_valid with "Hsi Hl")  as "%".
+
+    destruct_thread_step.
+    (* Thus, the reduction step must be a successful step. *)
+    eapply invert_step_resume in H; [ destruct H | eauto ]; subst.
+
+    (* Update the ghost heap. *)
+    iMod (gen_heap.gen_heap_update with "Hsi Hl") as "[Hsi Hl]".
+    ewp_mask_elim. iFrame.
+    rewrite try2_inject2_right.
+    iApply ("H" with "Hl").
+  Qed.
+
+End handle_rules.
+
 (* -------------------------------------------------------------------------- *)
 (** *Reasoning rules over effect handlers *)
 
@@ -205,11 +384,29 @@ Section handler_proof.
   Context `{!osirisGS Σ}.
 
   Context {A X : Type} `{Encode A}.
+  Context {E : coPset} {Ψ : iEff Σ} {ζ : exn → iProp Σ}.
 
   Import ewp_rules_tactics.
 
+  Lemma ewp_stop_perform {B X'} v k (Φ : outcome2 B X' → iProp Σ) :
+    Ψ allows perform v << λ w, ▷ ewp_def E (k w) Ψ Φ >> -∗
+    ewp_def E (Stop CPerf v k) Ψ Φ.
+  Proof.
+    iIntros "HP".
+    ewp_unfold_head.
+    by iModIntro.
+  Qed.
+
+  Lemma ewp_perform_inv {B X'} v k (Φ : outcome2 B X' → iProp Σ) :
+    ewp_def E (Stop CPerf v k) Ψ Φ ={E}=∗
+    Ψ allows perform v << λ w, ▷ ewp_def E (k w) Ψ Φ >>.
+  Proof.
+    ewp_unfold (Stop CPerf v k).
+    by iIntros ">HP !>".
+  Qed.
+
   (* Specification of [deep_handler] at the [expr] level. *)
-  Lemma imp_deep_handler `{Encode A'} E Ψ ζ (Φ : A → iProp Σ) Ψ' ζ' (Φ' : A' → iProp Σ) η e bs:
+  Lemma imp_deep_handler `{Encode A'} {Ψ'} {ζ'} {Φ' : A' → iProp Σ} (Φ : A → iProp Σ) η e bs:
     imp (eval η e) @ E <|Ψ|> ⟨⟨ ζ ⟩⟩ {{ Φ }} -∗
     (* The deep handler specification is met *)
     deep_handler_spec E Ψ ζ Φ η bs Ψ' ζ' Φ' -∗
@@ -222,7 +419,7 @@ Section handler_proof.
 
     deep_handler_spec_unfold.
     (* We proceed by Löb-induction after generalizing [η] [m] and [bs]. *)
-    iLöb as "IH" forall (m η bs Ψ' ζ' Φ' E).
+    iLöb as "IH" forall (m η bs Ψ' ζ' Φ').
 
     (* Expand the definition of [EWP] to inspect the possible steps that
         can result from [deep_handler η e bs]. *)
@@ -251,7 +448,7 @@ Section handler_proof.
       iDestruct "Hdh" as "[_ [_ Hdh]]".
 
       (* [Perform e] satisfies the protocol specification *)
-      iPoseProof (basic_rules.ewp_perform_inv with "[$]") as "HP"; iMod "HP".
+      iPoseProof (ewp_perform_inv with "[$]") as "HP"; iMod "HP".
 
       (* We allocate a new location that contains the continuation *)
       iDestruct (gen_heap.gen_heap_alloc _ _ (K k) with "Hsi")
@@ -259,10 +456,9 @@ Section handler_proof.
 
       iFrame.
       (* Install the handler around the location [l]. *)
-      simpl_wrap_eval_branches.
       ewp_mask_intro "Hmod".
       ewp_mask_elim.
-      iApply imp_wrap_deep.
+      iApply (imp_wrap_eval_branches (E:=E)).
       iIntros (?) "Hl".
       iSpecialize ("Hdh" $! e l').
 
@@ -273,13 +469,7 @@ Section handler_proof.
         iIntros "Hshot !>".
         rewrite deep_handler_spec_def_unfold.
         iSpecialize ("IH" with "Hk H").
-        iPoseProof (basic_rules.ewp_handle_inv with "HH IH") as "Hhandle".
-        iApply (imp_try2 (A1:=A') with "[Hhandle]"). rewrite /wrap_eval_branches seal_eq /pre_wrap_eval_branches /=.
-        iApply "Hhandle". iSplit.
-        - iIntros (a) "HΦ''".
-          iApply imp_ret; auto.
-        - iIntros (ex) "Hζ''".
-          iApply imp_throw; auto. }
+        iApply (ewp_handle_resume with "HH IH"). }
       iApply "Hdh". }
 
     { (* [StepHandleFork] *)
@@ -318,7 +508,7 @@ Section handler_proof.
       iApply ("IH" with "Hwp Hdh"). }
   Qed.
 
-  Lemma deep_handle_nil_ret η v E Ψ ζ (Φ : A → iProp Σ) :
+  Lemma deep_handle_nil_ret η v (Φ : A → iProp Σ) :
    imp match_failure () @ E <|Ψ|> ⟨⟨ ζ ⟩⟩ {{ Φ }} -∗
    imp (eval_branches η (O3Ret v) []) @ E <|Ψ|> ⟨⟨ ζ ⟩⟩ {{ Φ }}.
   Proof.
@@ -326,39 +516,39 @@ Section handler_proof.
     iApply "Hfail".
   Qed.
 
-  Lemma shallow_handle_nil_ret η v all_bs E Ψ ζ (Φ : A → iProp Σ) :
+  Lemma shallow_handle_nil_ret η v all_bs (Φ : A → iProp Σ) :
    imp match_failure () @ E <|Ψ|> ⟨⟨ ζ ⟩⟩ {{ Φ }} -∗
    imp (shallow_eval_branches η [] all_bs (O3Ret v)) @ E <|Ψ|> ⟨⟨ ζ ⟩⟩ {{ Φ }}.
   Proof.
     by iIntros; simpl_shallow_eval_branches.
   Qed.
 
-  Lemma deep_handle_nil_throw η e E Ψ ζ (Φ : A → iProp Σ) :
+  Lemma deep_handle_nil_throw η e (Φ : A → iProp Σ) :
    imp throw e @ E <|Ψ|> ⟨⟨ ζ ⟩⟩ {{ Φ }} -∗
    imp (eval_branches η (O3Throw e) []) @ E <|Ψ|> ⟨⟨ ζ ⟩⟩ {{ Φ }}.
   Proof.
     by iIntros; simpl_eval_branches.
   Qed.
 
-  Lemma shallow_handle_nil_throw η all_bs e E Ψ ζ (Φ : A → iProp Σ) :
+  Lemma shallow_handle_nil_throw η all_bs e (Φ : A → iProp Σ) :
     imp throw e @ E <|Ψ|> ⟨⟨ ζ ⟩⟩ {{ Φ }} -∗
     imp (shallow_eval_branches η [] all_bs (O3Throw e)) @ E <|Ψ|> ⟨⟨ ζ ⟩⟩ {{ Φ }}.
   Proof.
     by iIntros; simpl_shallow_eval_branches.
   Qed.
 
-  Lemma deep_handle_nil_perform {E} η eff k Ψ ζ (Φ : A → iProp Σ) :
+  Lemma deep_handle_nil_perform η eff k (Φ : A → iProp Σ) :
     Ψ allows perform eff << λ o, ▷ may_resume o k E Ψ ζ Φ >> -∗
     imp (eval_branches η (O3Perform eff k) []) @ E <|Ψ|> ⟨⟨ ζ ⟩⟩ {{ Φ }}.
   Proof.
     iIntros "Hk". simpl_eval_branches.
-    iApply basic_rules.ewp_stop_perform.
+    iApply imp_stop_perform.
     iApply (monotonic_prot with "[] Hk").
     iIntros (o) "Ho !>"; rewrite try2_inject2.
     iApply "Ho".
   Qed.
 
-  Lemma shallow_handle_nil_perform η eff k all_branches Ψ sk ζ (Φ : A → iProp Σ) :
+  Lemma shallow_handle_nil_perform η eff k all_branches sk (Φ : A → iProp Σ) :
     isCont k sk -∗
     Ψ allows perform eff
     << λ o,
@@ -366,31 +556,22 @@ Section handler_proof.
     imp (shallow_eval_branches η [] all_branches (O3Perform eff k)) <|Ψ|> ⟨⟨ ζ ⟩⟩ {{ Φ }}.
   Proof.
     iIntros "Hk Hperf". simpl_shallow_eval_branches.
-    iApply imp_wrap_shallow.
+    iApply imp_bind.
+    { iApply imp_wrap_shallow. iIntros (?) "Hcont". iExact "Hcont". }
 
-    iIntros (l) "Hl". iNext. cbn.
+    iIntros (l) "Hl".
 
     iApply imp_stop_perform.
 
-    rewrite /prot /iEff_car.
-    iApply (monotonic_prot (Ψ:=upcl Ψ) with "[Hl]").
-    { iIntros (o) "H".
-      iNext. rewrite try2_inject2.
-      iApply (imp_resume with "Hl"). rewrite try2_inject2_right.
-      iIntros "_".
-      iApply (bi.later_mono with "H").
-      iIntros "H".
-      unfold stop.
-      iApply "H". }
-    iApply (monotonic_prot (Ψ:=upcl Ψ) with "[Hk]").
-    { iIntros (o) "H".
-      iPoseProof (basic_rules.ewp_handle_inv with "Hk") as "Hcov".
-      unfold cont; simpl.
-      iApply "Hcov". iApply "H". }
-    done.
+    iApply (monotonic_prot with "[Hl Hk] Hperf").
+    iIntros (o) "HHandle !>".
+    rewrite try2_inject2.
+    iApply (imp_resume with "Hl").
+    iIntros "Hshot !>".
+    iApply (ewp_handle_resume with "Hk HHandle").
   Qed.
 
-  Lemma deep_handle_cons η o cp e bs E Ψ ζ (Φ : A → iProp Σ) Hη φ :
+  Lemma deep_handle_cons η o cp e bs (Φ : A → iProp Σ) Hη φ :
     ⌜cpattern η η cp o Hη φ⌝ -∗
     (∀ η, ⌜Hη η⌝ -∗ imp (eval η e) @ E <|Ψ|> ⟨⟨ ζ ⟩⟩ {{ Φ }}) ∧
     (⌜φ⌝ -∗ imp (eval_branches η o bs) @ E <| Ψ |> ⟨⟨ ζ ⟩⟩ {{ Φ }}) -∗
@@ -403,7 +584,7 @@ Section handler_proof.
     - iApply "Hmono". iFrame "%".
   Qed.
 
-  Lemma deep_handle_cons_skip η o cp e bs E Ψ ζ (Φ : A → iProp Σ) :
+  Lemma deep_handle_cons_skip η o cp e bs (Φ : A → iProp Σ) :
     valid_cpattern_match cp o = false →
     imp (eval_branches η o bs) @ E <| Ψ |> ⟨⟨ ζ ⟩⟩ {{ Φ }} -∗
     imp (eval_branches η o (Branch cp e :: bs)) @ E <| Ψ |> ⟨⟨ ζ ⟩⟩ {{ Φ }}.
