rocq-osiris/theories/program_logic/rules/atomic_rules.v
@@ -1,0 +1,190 @@
+From iris.proofmode Require Import proofmode.
+From iris.base_logic.lib Require Import gen_heap invariants.
+
+From osiris.lang Require Import lang.
+From osiris.tactics Require Import osiris_utils.
+From osiris.program_logic Require Import thread_step ewp tactics.
+From osiris.program_logic.rules Require Import impure_rules stop_rules.
+
+Import ewp_rules_tactics.
+
+Instance crash_atomic {V X} :
+  thread_step.Atomic (@Crash V X).
+Proof. constructor. inversion H; subst. inversion H1. Qed.
+
+Global Instance load_atomic l :
+  thread_step.Atomic (load l).
+Proof.
+  unfold thread_step.Atomic. intros.
+
+  destruct_thread_step.
+  unfold step_load_2.
+  destruct (σ' !! l) as [ [| |] | ]; by econstructor.
+Qed.
+
+Global Instance eload_atomic η p :
+  thread_step.Atomic (eval η (ELoad (EPath p))).
+Proof.
+  simpl_eval.
+  destruct (lookup_path η p); last apply _.
+  destruct v; simpl; try (rewrite bind_crash; apply _).
+  apply _.
+Qed.
+
+Global Instance store_atomic l v :
+  thread_step.Atomic (code.store l v).
+Proof.
+  unfold thread_step.Atomic. intros.
+
+  destruct_thread_step.
+  unfold step_store_2.
+  destruct (σ !! l0) as [ [| |] | ]; by econstructor.
+Qed.
+
+Global Instance cas_atomic l seen v' :
+  thread_step.Atomic (cas l seen v').
+Proof.
+  unfold thread_step.Atomic. intros.
+
+  destruct_thread_step.
+  unfold step_cas_2.
+  destruct (σ !! l0) as [ [| |] | ]; try by econstructor.
+  destruct (phys_eq_val _ _) as [ [|] | ]; by econstructor.
+Qed.
+
+
+Section imp_atomic_rules.
+
+  Context `{!osirisGS Σ}.
+  Context {Ψ : iEff Σ} {ζ : exn → iProp Σ}.
+
+  Lemma imp_store_atomic `{Encode A} (E2 E1 : coPset) η e1 e2 (Φ1 : loc → _) (Φ2 : A → _) (Φ : () → _) :
+    impure E1 (eval η e1) Ψ ζ Φ1 -∗
+    impure E1 (eval η e2) Ψ ζ Φ2 -∗
+    ▷ (|={E1,E2}=>
+         ∀ l x, Φ1 l -∗ Φ2 x -∗
+                ∃ v, ▷ l ↦ v ∗
+                     ▷ (l ↦ #x -∗ |={E2,E1}=> Φ ())) -∗
+    impure E1 (eval η (EStore e1 e2)) Ψ ζ Φ.
+  Proof.
+    iIntros "He1 He2 Hstore".
+    simpl_eval.
+    iApply (imp_bind (A1:=loc * A) with "[-]").
+    set_postcondition
+      (λ '((l, x) : loc * A),
+         |={E1,E2}=> ∃ v, ▷ l ↦ v ∗
+                          ▷ (l ↦ #x -∗ |={E2,E1}=> Φ ()))%I.
+    { iApply (imp_Par with "[He1] He2").
+      { iApply (imp_as_loc with "He1"). }
+      iSplit.
+      - iIntros (e) "He !>". iApply (imp_throw with "He").
+      - iIntros (l x) "HΦ1 HΦ2 !>".
+        iApply imp_ret. instantiate (1:=(_,_)). encode.
+        iMod "Hstore". iModIntro.
+        iDestruct ("Hstore" with "HΦ1 HΦ2") as "(%v & $ & $)". }
+    iIntros ((l & x)) "Hl /=".
+    iApply (imp_atomic' E1 E2).
+    iMod "Hl" as "(%v & Hl & Hstore)".
+    iApply (imp_store' with "Hl").
+    iApply "Hstore".
+  Qed.
+
+  Lemma imp_cas_atomic `{PhysEqDec A} (E2 E1 : coPset) η e1 e2 e3 (Φ1 : loc → _) (Φ2 Φ3 : A → _) (Φ : bool → _) :
+    impure E1 (eval η e1) Ψ ζ Φ1 -∗
+    impure E1 (eval η e2) Ψ ζ Φ2 -∗
+    impure E1 (eval η e3) Ψ ζ Φ3 -∗
+    ▷ (|={E1,E2}=>
+         ∀ l seen v',
+         Φ1 l -∗ Φ2 seen -∗ Φ3 v' -∗
+         ∃ v, ▷ l ↦ #v ∗
+              ▷ (l ↦ (if phys_eq_val_ v seen then #v' else #v) -∗
+                 |={E2,E1}=> Φ (phys_eq_val_ v seen))) -∗
+    impure E1 (eval η (ECAS e1 e2 e3)) Ψ ζ Φ.
+  Proof.
+    iIntros "He1 He2 He3 Hcas".
+    simpl_eval.
+    iApply (imp_bind (A1:=loc * A * A) with "[-]").
+    set_postcondition
+      (λ '((l, seen, v') : loc * A * A),
+         |={E1,E2}=> ∃ v, ▷ l ↦ #v ∗
+                          ▷ (l ↦ (if phys_eq_val_ v seen then #v' else #v) -∗
+                             |={E2,E1}=> Φ (phys_eq_val_ v seen)))%I.
+    { iApply (imp_Par (A1:=loc * A) with "[He1 He2] He3").
+      { iApply (imp_Par with "[He1] He2").
+        { iApply (imp_as_loc with "He1"). }
+        iSplit.
+        - iIntros (e) "He !>". iApply (imp_throw with "He").
+        - iIntros (l x) "HΦ1 HΦ2 !>".
+          set_postcondition (λ '(l, x), Φ1 l ∗ Φ2 x)%I.
+          iApply imp_ret. instantiate (1:=(_,_)). encode.
+          iFrame. }
+      iSplit.
+      - iIntros (e) "He !>". iApply (imp_throw with "He").
+      - iIntros ((l & seen) x) "(HΦ1 & HΦ2) HΦ3".
+        iApply imp_ret. instantiate (1:=((_,_),_)). encode.
+        iNext. iMod "Hcas". iModIntro.
+        iDestruct ("Hcas" with "HΦ1 HΦ2 HΦ3") as "(%v & $ & $)". }
+    iIntros (((l & seen) & x)) "Hcas /=".
+    iApply (imp_atomic' E1 E2).
+    iMod "Hcas" as "(%v & Hl & Hcas)".
+    iApply (imp_cas with "Hl Hcas").
+  Qed.
+
+End imp_atomic_rules.
+
+Section imp_inv_rules.
+
+  Context `{!osirisGS Σ}.
+  Context {E : coPset} {Ψ : iEff Σ} {ζ : exn → iProp Σ}.
+  Context {N : namespace} {P : iProp Σ}.
+
+  Lemma imp_store_inv `{Encode A} η e1 e2 (Φ1 : loc → _) (Φ2 : A → _) (Φ : () → _) :
+    ↑N ⊆ E →
+    inv N P -∗
+    impure E (eval η e1) Ψ ζ Φ1 -∗
+    impure E (eval η e2) Ψ ζ Φ2 -∗
+    (▷ ∀ l x, Φ1 l -∗ Φ2 x -∗
+              ▷ P -∗
+              ∃ v, ▷ l ↦ v ∗
+                   ▷ (l ↦ #x -∗ ▷ P ∗ Φ ())) -∗
+    impure E (eval η (EStore e1 e2)) Ψ ζ Φ.
+  Proof.
+    iIntros (Hsubset) "#Hinv He1 He2 Hstore".
+    iApply (imp_store_atomic (E ∖ ↑N) with "He1 He2").
+    iNext.
+    iPoseProof (inv_acc with "Hinv") as ">[HP HClose]". assumption.
+    iIntros "!>" (l x) "HΦ1 HΦ2".
+    iDestruct ("Hstore" with "HΦ1 HΦ2 HP") as "(% & $ & Hstore)".
+    iIntros "!> Hl".
+    iDestruct ("Hstore" with "Hl") as "[HP HΦ]".
+    iMod ("HClose" with "HP").
+    iApply "HΦ".
+  Qed.
+
+  Lemma imp_CAS_inv `{PhysEqDec A} η e1 e2 e3 (Φ1 : loc → _) (Φ2 Φ3 : A → _) (Φ : bool → _) :
+    ↑N ⊆ E →
+    inv N P -∗
+    impure E (eval η e1) Ψ ζ Φ1 -∗
+    impure E (eval η e2) Ψ ζ Φ2 -∗
+    impure E (eval η e3) Ψ ζ Φ3 -∗
+    (▷ ∀ l seen v',
+       Φ1 l -∗ Φ2 seen -∗ Φ3 v' -∗
+       ▷ P -∗
+       ∃ v, ▷ l ↦ #v ∗
+            ▷ (l ↦ (if phys_eq_val_ v seen then #v' else #v) -∗
+               ▷ P ∗ Φ (phys_eq_val_ v seen))) -∗
+    impure E (eval η (ECAS e1 e2 e3)) Ψ ζ Φ.
+  Proof.
+    iIntros (Hsubset) "#Hinv He1 He2 He3 Hcas".
+    iApply (imp_cas_atomic (E ∖ ↑N) with "He1 He2 He3").
+    iNext.
+    iPoseProof (inv_acc with "Hinv") as ">[HP HClose]". assumption.
+    iIntros "!>" (l seen v') "HΦ1 HΦ2 HΦ3".
+    iDestruct ("Hcas" with "HΦ1 HΦ2 HΦ3 HP") as "(% & $ & Hcas)".
+    iIntros "!> Hl".
+    iDestruct ("Hcas" with "Hl") as "[HP HΦ]".
+    iMod ("HClose" with "HP").
+    iApply "HΦ".
+  Qed.
+
+End imp_inv_rules.
