rocq-osiris/theories/program_logic/rules/auxiliary_rules.v
@@ -1,0 +1,285 @@
+From iris.proofmode Require Import proofmode.
+
+From osiris Require Import lang.
+From osiris.program_logic Require Import ewp.
+From osiris.program_logic.rules Require Import impure_rules stop_rules.
+
+From osiris.program_logic.pure Require Import pattern_rules.
+
+Section imp_eval.
+
+  Context `{!osirisGS Σ}.
+  Context {E : coPset} {Ψ : iEff Σ} {ζ : exn → iProp Σ}.
+
+  Lemma imp_module sitems {Q : env -> iProp Σ} η :
+    imp (eval_sitems (η, []) sitems) @ E <|Ψ|> ⟨⟨ ζ ⟩⟩ {{ λ '((_, δ) : envs), Q δ }} -∗
+    imp (eval_mexpr η (MStruct sitems)) @ E <|Ψ|> ⟨⟨ ζ ⟩⟩ {{ Q }}.
+  Proof.
+    iIntros "Hsitems".
+    simpl_eval_mexpr.
+    iApply (imp_bind with "Hsitems").
+    iIntros ([η' δ']) "HQ".
+    iApply (imp_ret with "HQ"). encode.
+  Qed.
+
+  Lemma imp_sitems_cons {Q : envs → iProp Σ} (φ : envs → iProp Σ) sitem sitems (ηδ : envs) :
+    imp (eval_sitem ηδ sitem) @ E <|Ψ|> ⟨⟨ ζ ⟩⟩ {{ φ }} -∗
+    (∀ ηδ, φ ηδ -∗ imp eval_sitems ηδ sitems @ E <| Ψ |> ⟨⟨ ζ ⟩⟩ {{ Q }}) -∗
+    imp (eval_sitems ηδ (sitem :: sitems)) @ E <|Ψ|> ⟨⟨ ζ ⟩⟩ {{ Q }}.
+  Proof.
+    iIntros "Hsitem Hcov".
+    simpl_eval_sitems. iApply (imp_bind with "Hsitem").
+    iIntros ([η' δ']) "Hφ".
+    iApply ("Hcov" with "Hφ").
+  Qed.
+
+  Lemma imp_sitems_nil Q ηδ :
+    Q ηδ -∗
+    imp eval_sitems ηδ [] @ E <| Ψ |> ⟨⟨ ζ ⟩⟩ {{ Q }}.
+  Proof.
+    simpl_eval_sitems.
+    iIntros "HQ". destruct ηδ.
+    by iApply (imp_ret with "HQ").
+  Qed.
+
+  Lemma imp_sitem_letrec_singleton (spec : val → iProp Σ) x af (η δ : env) :
+    spec (VCloRec η [RecBinding x af] x) -∗
+    imp (eval_sitem (η, δ) (ILetRec [RecBinding x af])) @ E <|Ψ|> ⟨⟨ ζ ⟩⟩ {{
+          λ '(η0, δ0),
+            ∃ clo, spec clo ∧ ⌜η0 = (x, clo) :: η⌝ ∧ ⌜δ0 = (x, clo) :: δ⌝
+      }}.
+  Proof.
+    iIntros "Hspec".
+    simpl_eval_sitem.
+    iApply imp_ret. instantiate (1:=(_,_)). reflexivity.
+    iExists _. iFrame.
+    iSplit; iPureIntro; reflexivity.
+  Qed.
+
+  Lemma imp_sitems_letrec sitems (spec : val → iProp Σ) x af (η δ : env) Q :
+    spec (VCloRec η [RecBinding x af] x) -∗
+    (∀ v, spec v -∗ imp (eval_sitems ((x, v) :: η, (x, v) :: δ) sitems) @ E <|Ψ|>
+      ⟨⟨ζ⟩⟩ {{ Q }}) -∗
+    imp (eval_sitems (η, δ) ((ILetRec [RecBinding x af]) :: sitems)) @ E <|Ψ|>
+      ⟨⟨ζ⟩⟩ {{ Q }}.
+  Proof.
+    iIntros "Hspec Hcov".
+    iApply (imp_sitems_cons with "[Hspec]").
+    { iApply (imp_sitem_letrec_singleton with "Hspec"). }
+    iIntros ([??]) "(% & Hspec & [-> ->])".
+    iApply ("Hcov" with "Hspec").
+  Qed.
+
+  Lemma imp_struct_let bs (Q : envs → iProp Σ) (Q' : env → iProp Σ) η δ :
+    imp (eval_bindings η bs) @ E <| Ψ |> ⟨⟨ ζ ⟩⟩ {{ Q' }} -∗
+    (∀ η', Q' η' -∗ Q (η' ++ η, η' ++ δ)) -∗
+    imp (eval_sitem (η, δ) (ILet bs)) @ E <| Ψ |> ⟨⟨ ζ ⟩⟩ {{ Q }}.
+  Proof.
+    iIntros "Hbindings Hmono".
+    simpl_eval_sitem.
+    iApply (imp_bind with "Hbindings").
+    iIntros (η') "HQ'".
+    iApply imp_ret; first (instantiate (1:=(_,_)); encode).
+    iApply ("Hmono" with "HQ'").
+  Qed.
+
+  Lemma imp_bindings_cons `{Encode A} (Φ : A → iProp Σ) η e bs Q P p :
+    imp eval η e @ E <| Ψ |> ⟨⟨ ζ ⟩⟩ {{ Φ }} -∗
+    (∀ (a : A), Φ a -∗ ⌜pattern η [] p #a (P a) False⌝) -∗
+    imp eval_bindings η bs @ E <| Ψ |> ⟨⟨ ζ ⟩⟩ {{ Q }} -∗
+    imp eval_bindings η (Binding p e :: bs) @ E <| Ψ |> ⟨⟨ ζ ⟩⟩
+      {{ λ η, ∃ a η' δ', ⌜η = η' ++ δ'⌝ ∗ Φ a ∗ ⌜P a η'⌝ ∗ Q δ' }}.
+  Proof.
+    iIntros "He Hpat Hbs".
+    simpl_eval_bindings.
+    iApply (imp_Par with "[He Hpat] Hbs").
+    { iApply (imp_bind with "He").
+      iIntros (?) "HΦ". iApply imp_widen.
+      iDestruct ("Hpat" with "HΦ") as "%Hpat".
+      unfold pattern in Hpat. simpl.
+      destruct (eval_pat η [] p #x).
+      - instantiate (1 := (λ η, ∃ x, Φ x ∗ ⌜P x η⌝)%I).
+        iFrame. iFrame "%". auto.
+      - contradiction. }
+    iSplit.
+    { iIntros (?) "Hζ !>".
+      iApply (imp_throw with "Hζ"). }
+    iIntros (x η') "(%a & HΦ & HP) Hη".
+    iNext. rewrite /continue. simpl.
+    iApply imp_ret. reflexivity.
+    iFrame. auto.
+  Qed.
+
+  Lemma imp_bindings_nil η :
+    ⊢ imp eval_bindings η [] @ E <|Ψ|> ⟨⟨ ζ ⟩⟩ {{ λ η, ⌜η = []⌝ }}.
+  Proof.
+    simpl_eval_bindings.
+    iApply imp_ret. reflexivity. auto.
+  Qed.
+
+  Lemma imp_bind_var `{Encode A} (Φ : A → iProp Σ) η e name :
+    imp eval η e @ E <|Ψ|> ⟨⟨ ζ ⟩⟩ {{ Φ }} -∗
+    imp eval_bindings η [Binding (PVar name) e] @ E <| Ψ |> ⟨⟨ ζ ⟩⟩
+          {{ λ (η' : env), ∃ a : A, Φ a ∧ ⌜η' = [(name, #a)]⌝ }}.
+  Proof.
+    iIntros "HSpec".
+    iApply (imp_wand with "[HSpec]").
+    { iApply (imp_bindings_cons with "HSpec").
+      - iIntros (a) "HΦ".
+        iPureIntro; apply pat_PVar.
+        instantiate (1:=(λ a η, η = [(name, #a)])).
+        reflexivity.
+      - iApply imp_bindings_nil. }
+    iIntros (η') "(%a & % & % & -> & HΦ & -> & ->)".
+    iFrame. auto.
+  Qed.
+
+  Lemma imp_struct_let_single `{Encode A} (spec : A → iProp Σ) name e (η δ : env) :
+    imp (eval η e) @ E <| Ψ |> ⟨⟨ ζ ⟩⟩ {{ spec }} -∗
+    imp (eval_sitem (η, δ) (ILet [Binding (PVar name) e])) @ E <|Ψ|> ⟨⟨ ζ ⟩⟩ {{
+          λ '(η', δ'),
+            ∃ a : A, spec a ∧ ⌜η' = (name, #a) :: η ∧ δ' = (name, #a) :: δ⌝
+      }}.
+  Proof.
+    iIntros "Hspec".
+    iApply (imp_struct_let with "[Hspec]").
+    { iApply (imp_bind_var with "Hspec"). }
+    iIntros (?) "(%a & Hspec & ->)".
+    iFrame. iPureIntro; split; reflexivity.
+  Qed.
+
+  Lemma imp_sitem_extend es (Q : envs -> iProp Σ) (η δ : env) :
+    imp eval_type_extensions es @ E <|Ψ|> ⟨⟨ ζ ⟩⟩ {{ λ (δ' : env), Q (δ' ++ η, δ' ++ δ) }} -∗
+    imp eval_sitem (η,δ) (IExtend es) @ E <| Ψ |> ⟨⟨ ζ ⟩⟩ {{ Q }}.
+  Proof.
+    iIntros "Hes".
+    simpl_eval_sitem.
+    iApply (imp_bind _ _ (λ δ', ret (δ' ++ η, δ' ++ δ)) with "Hes").
+    iIntros (η') "HQ".
+    iApply (imp_ret with "HQ"); reflexivity.
+  Qed.
+
+  Lemma imp_sitems_extend sitems x Q η δ :
+    (∀ l, l ↦ #() -∗
+          imp eval_sitems ((x, VLoc l) :: η, (x, VLoc l) :: δ) sitems @ E <| Ψ |> ⟨⟨ ζ ⟩⟩ {{ Q }}) -∗
+    imp eval_sitems (η,δ) ((IExtend [x]) :: sitems) @ E <| Ψ |> ⟨⟨ ζ ⟩⟩ {{ Q }}.
+  Proof.
+    iIntros "Hcov".
+    iApply (imp_sitems_cons).
+    { iApply (imp_sitem_extend).
+      iApply imp_bind. iApply imp_alloc.
+      iIntros (l) "Hl"; simpl; iApply imp_ret. reflexivity.
+      Unshelve.
+      2: (apply (λ ηδ,
+                   (∃ l, ⌜ηδ = ((x, VLoc l) :: η, (x, VLoc l):: δ)⌝ ∗ l ↦ VUnit)%I)).
+      simpl.
+      iExists l; iFrame. iPureIntro; reflexivity. }
+    iIntros ([??]) "(% & -> & Hl)".
+    iApply ("Hcov" with "Hl").
+  Qed.
+
+  Lemma imp_sitem_open me Q φ (η δ : env) :
+    imp eval_mexpr η me @ E <| Ψ |> ⟨⟨ ζ ⟩⟩ {{ φ }} -∗
+    ( ∀ δ', φ δ' -∗ Q (δ' ++ η, δ) ) -∗
+    imp eval_sitem (η, δ) (IOpen me) @ E <| Ψ |> ⟨⟨ ζ ⟩⟩ {{ Q }}.
+  Proof.
+    iIntros "Hme Hcov". simpl_eval_sitem.
+    iApply (imp_bind with "[Hme]").
+    { iApply (imp_as_struct with "Hme"). }
+    iIntros (η') "Hφ".
+    iApply imp_ret; first (instantiate (1:=(_,_)); encode).
+    iApply ("Hcov" with "Hφ").
+  Qed.
+
+  Lemma imp_sitem_module m me Q (φ : env → iProp Σ) (η δ : env) :
+    imp eval_mexpr η me @ E <| Ψ |> ⟨⟨ ζ ⟩⟩ {{ φ }} -∗
+    ( ∀ δ', φ δ' -∗ Q ((m, #δ') :: η, (m, #δ') :: δ) ) -∗
+    imp eval_sitem (η, δ) (IModule m me) @ E <| Ψ |> ⟨⟨ ζ ⟩⟩ {{ Q }}.
+  Proof.
+    iIntros "Hme Hcov". simpl_eval_sitem.
+    iApply (imp_bind with "Hme").
+    iIntros (η') "Hφ".
+    iApply imp_ret; first (instantiate (1:=(_,_)); encode).
+    iApply ("Hcov" with "Hφ").
+  Qed.
+
+  Lemma imp_sitems_module {m me sitems Q} (φ : env → iProp Σ) (η δ : env) :
+    imp eval_mexpr η me @ E <| Ψ |> ⟨⟨ ζ ⟩⟩ {{ φ }} -∗
+    ( ∀ δ', φ δ' -∗ imp eval_sitems ((m, #δ') :: η, (m, #δ') :: δ) sitems @ E <| Ψ |> ⟨⟨ ζ ⟩⟩ {{ Q }}) -∗
+    imp eval_sitems (η, δ) ((IModule m me) :: sitems) @ E <| Ψ |> ⟨⟨ ζ ⟩⟩ {{ Q }}.
+  Proof.
+    iIntros "Hme Hcov".
+    iApply (imp_sitems_cons with "[Hme]").
+    { iApply (imp_sitem_module with "Hme").
+      iIntros (δ') "Hφ".
+      instantiate (1 := (λ ηδ, ∃ δ', φ δ' ∗ ⌜ηδ = (_,_)⌝)%I).
+      iFrame. auto. }
+    iIntros (?) "(% & Hφ & ->)".
+    iApply ("Hcov" with "Hφ").
+  Qed.
+
+  Lemma imp_type_extension_cons e es Q :
+    ▷ (∀ l, l ↦ #() -∗
+            imp eval_type_extensions es @ E <| Ψ |> ⟨⟨ ζ ⟩⟩ {{ λ δ, Q ((e, VLoc l) :: δ) }}) -∗
+    imp eval_type_extensions (e :: es) @ E <| Ψ |> ⟨⟨ ζ ⟩⟩ {{ Q }}.
+  Proof.
+    iIntros "Hes". simpl.
+    iApply (imp_bind with "[Hes]").
+    { iApply imp_alloc'. iIntros "!>" (l) "Hl".
+      iSpecialize ("Hes" with "Hl").
+      iExact "Hes". }
+    iIntros (l) "Hes".
+    iApply (imp_bind with "Hes").
+    iIntros (η) "HQ".
+    iApply (imp_ret with "HQ"). reflexivity.
+  Qed.
+
+  Lemma imp_type_extension_nil :
+    ⊢ imp eval_type_extensions [] @ E <| Ψ |> ⟨⟨ ζ ⟩⟩ {{ λ η, ⌜η = []⌝ }}.
+  Proof. simpl. by iApply imp_ret. Qed.
+
+  Lemma imp_let `{Encode A} (spec : A → iProp Σ) x e Q η δ :
+    imp eval η e @ E <| Ψ |> ⟨⟨ ζ ⟩⟩ {{ spec }} -∗
+    (∀ a, spec a -∗ Q ((x, #a) :: η, (x, #a) :: δ)) -∗
+    imp eval_sitem (η, δ) (ILet [Binding (PVar x) e]) @ E <| Ψ |> ⟨⟨ ζ ⟩⟩ {{ Q }}.
+  Proof.
+    iIntros "He HQ".
+    iApply (imp_wand _ (eval_sitem (η, δ) (ILet [Binding (PVar x) e])) with "[He]").
+    iApply (imp_struct_let_single with "He").
+    iIntros ([η' δ']) "(%a & Ha & -> & ->)".
+    iApply ("HQ" with "Ha").
+  Qed.
+
+  Lemma imp_sitems_let `{Encode A} (spec : A → iProp Σ) sitems x e Q η δ :
+    imp eval η e @ E <| Ψ |> ⟨⟨ ζ ⟩⟩ {{ spec }} -∗
+      (∀ a, spec a -∗
+            imp eval_sitems ((x, #a) :: η, (x, #a) :: δ) sitems @ E <| Ψ |> ⟨⟨ ζ ⟩⟩ {{ Q }}) -∗
+      imp eval_sitems (η, δ) ((ILet [Binding (PVar x) e])::sitems) @ E <| Ψ |> ⟨⟨ ζ ⟩⟩ {{ Q }}.
+  Proof.
+    iIntros "He Hcov".
+    iApply (imp_sitems_cons with "[He]").
+    iApply (imp_let with "He").
+    instantiate (1 := (λ ηδ, ∃ a, spec a ∗ ⌜ηδ = (x ~> #a; η, x ~> #a; δ)⌝)%I).
+    iIntros (a) "Ha". iFrame. auto.
+    iIntros (ηδ) "(%a & Ha & ->)".
+    iApply ("Hcov" with "Ha").
+  Qed.
+
+  Lemma imp_sitems_external Φ sitems x e Q η δ :
+    imp eval [] e @ E <| Ψ |> ⟨⟨ ζ ⟩⟩ {{ Φ }} -∗
+    (∀ v, Φ v -∗ imp eval_sitems ((x, v) :: η, (x, v) :: δ) sitems @ E <| Ψ |> ⟨⟨ ζ ⟩⟩ {{ Q }}) -∗
+    imp eval_sitems (η, δ) ((IExternal x e)::sitems) @ E <| Ψ |> ⟨⟨ ζ ⟩⟩ {{ Q }}.
+  Proof.
+    iIntros "He Hcov".
+    iApply (imp_sitems_cons with "[He]").
+    { simpl_eval_sitem.
+      instantiate (1 := (λ ηδ, ∃ x0, ⌜ηδ = (x ~> x0; η, x ~> x0; δ)⌝ ∗ Φ x0)%I).
+      iApply (imp_bind with "He").
+      iIntros (?) "HΦ".
+      iApply imp_ret; first (instantiate (1:=(_,_)); encode).
+      by iFrame. }
+    iIntros (?) "(% & -> & HΦ)".
+    iApply ("Hcov" with "HΦ").
+  Qed.
+
+End imp_eval.
