rocq-osiris/theories/program_logic/rules/micro_rules.v
@@ -1,0 +1,363 @@
+From iris.proofmode Require Import proofmode.
+From iris.base_logic.lib Require Import gen_heap.
+
+From osiris Require Import base.
+From osiris.lang Require Import lang.
+From osiris.semantics Require Import semantics.
+From osiris.program_logic Require Import thread_step ewp tactics.
+
+From osiris.program_logic.rules Require Import basic_rules.
+
+Import ewp_rules_tactics.
+
+(* ------------------------------------------------------------------------ *)
+
+Section ewp_basic_rules.
+
+  Context `{!osirisGS Σ}.
+  Import ewp_rules_tactics.
+
+  Context {A X : Type}.
+  Context {E : coPset} {Ψ : iEff Σ} {Q : outcome2 A X → iProp Σ}.
+
+  Implicit Type m : micro A X.
+
+  (* Values *)
+  Lemma ewp_ret v :
+    Q (O2Ret v) -∗ ewp_def E (ret v : micro A X) Ψ Q.
+  Proof. iIntros "HΦ". by rewrite ewp_unfold /ewp_pre. Qed.
+
+  Lemma ewp_ret_inv v :
+    ewp_def E (Ret v : micro A X) Ψ Q ={E}=∗ Q (O2Ret v).
+  Proof.
+    iIntros "HRet".
+    by rewrite ewp_unfold /ewp_pre.
+  Qed.
+
+  Lemma ewp_throw (e : X) :
+    Q (O2Throw e) -∗ ewp_def E (Throw e : micro A X) Ψ Q.
+  Proof. iIntros "Hζ". by rewrite ewp_unfold /ewp_pre. Qed.
+
+  Lemma ewp_throw_inv v :
+    ewp_def E (Throw v : micro A X) Ψ Q ={E}=∗ Q (O2Throw v).
+  Proof.
+    iIntros "HThrow".
+    by rewrite ewp_unfold /ewp_pre.
+  Qed.
+
+  Lemma ewp_crash_inv :
+    ewp_def E (Crash : micro A X) Ψ Q ={E}=∗ False.
+  Proof.
+    ewp_unfold (@Crash A X).
+    by iIntros "Hsi".
+  Qed.
+
+  Lemma ewp_outcome2 o :
+    Q o -∗ ewp_def E (inject2 o : micro A X) Ψ Q.
+  Proof.
+    iIntros "HΦ". destruct o; simpl.
+    - by iApply ewp_ret.
+    - by iApply ewp_throw.
+  Qed.
+
+  Lemma ewp_outcome2_inv o :
+    ewp_def E (inject2 o : micro A X) Ψ Q ={E}=∗ Q o.
+  Proof.
+    iIntros "Hv".
+    ewp_unfold (inject2 o); by destruct o.
+  Qed.
+
+  Lemma ewp_outcome2_fupd o :
+    (|={E}=> Q o) -∗ ewp_def E (inject2 o : micro A X) Ψ Q.
+  Proof.
+    iIntros "HΦ".
+    rewrite ewp_unfold /ewp_pre.
+    by destruct o.
+  Qed.
+
+End ewp_basic_rules.
+
+(* ------------------------------------------------------------------------ *)
+(* Invert cases where there are premises of the form
+          [EWP (ret _) _] [EWP crash _] or [EWP (throw _) _] *)
+
+Ltac ewp_invert :=
+  lazymatch goal with
+  (* EWP throw *)
+  | |- context [environments.Esnoc _ ?Hwp (ewp_def _ (throw _) _ _)] =>
+      iPoseProof (ewp_throw_inv with "[$]") as "HΦ"
+  (* EWP ret *)
+  | |- context [environments.Esnoc _ ?Hwp (ewp_def _ (ret _) _ _)] =>
+      iPoseProof (ewp_ret_inv with "[$]") as "HΦ"
+  (* EWP crash *)
+  | |- context [environments.Esnoc _ ?Hwp (ewp_def _ Crash _ _)] =>
+      iMod (ewp_crash_inv with "[$]") as "%"
+  | |- context [environments.Esnoc _ ?Hwp (ewp_def _ (crash _) _ _)] =>
+      iMod (ewp_crash_inv with "[$]") as "%"
+  end.
+
+(* -------------------------------------------------------------------------- *)
+
+(* Effect and handler rules *)
+
+Section ewp_rules.
+
+  Context `{!osirisGS Σ}.
+
+  Context {A X : Type}.
+  Context {ι : thread} {E : coPset} {Ψ : iEff Σ} {Q : outcome2 A X → iProp Σ}.
+
+  Implicit Type m : micro A X.
+  Import ewp_rules_tactics.
+
+  Lemma is_ewp_case_try2_None {B X'} m (f : _ -> micro B X'):
+    is_ewp_case m = WPStep ->
+    is_ewp_case (try2 m f) = WPStep.
+  Proof.
+    intros Hm. destruct m; inversion Hm; try done.
+    destruct c; inversion H0; try done.
+  Qed.
+
+  Lemma is_ewp_case_try_None {B X'} m (f : A -> micro B X') (h : X -> micro B X'):
+    is_ewp_case m = WPStep ->
+    is_ewp_case (try m f h) = WPStep.
+  Proof.
+    intros Hm.
+    unfold try.
+    by apply is_ewp_case_try2_None.
+  Qed.
+
+  (* ------------------------------------------------------------------------ *)
+  (** *Try rule *)
+
+  Lemma ewp_try2 {B X'} m (f : _-> micro B X') Φ :
+    ewp_def E m Ψ (λ o, ewp_def E (f o) Ψ Φ) -∗
+    ewp_def E (try2 m f) Ψ Φ.
+  Proof.
+    iIntros "Hwp".
+    iLöb as "IH" forall (m).
+    ewp_case m.
+    (* Case: [m1] is an outcome2. *)
+    (* The result is immediate. *)
+    { rewrite try2_inject2.
+      iPoseProof (ewp_outcome2_inv with "Hwp") as "Hret"; cbn.
+      iApply (fupd_ewp with "Hret"). }
+    (* Case : [m1] is [crash]; trivial  *)
+    { iClear "IH".
+      iApply fupd_ewp.
+      ewp_unfold (@Crash A X); by iMod "Hwp". }
+    (* Case : [m1] is [Perform _ _]. *)
+    { cbn.
+      ewp_unfold_all.
+      iMod "Hwp"; iModIntro.
+      iApply (monotonic_prot with "[-Hwp] Hwp").
+      iIntros (o) "Hwp !>".
+      iApply ("IH" with "Hwp"). }
+    { (* If [m] can step, then so can [try m f h]. *)
+      pose proof (is_ewp_case_try2_None m f Hhm) as Hhm2.
+      ewp_unfold_all. rewrite Hhm. rewrite Hhm2.
+      (* Process a step of computation. *)
+      intro_state. spec_state.
+      iModIntro. apply invert_can_progress in Hstep.
+      destruct Hstep as [ Hstep | Hstep ].
+      { (* Case: [m1] is [Join _]. *)
+        destruct Hstep as (ι' & k & -> & Hdom).
+        discriminate.  }
+      destruct Hstep as [ Hstep | Hstep ].
+      { (* Case: [m1] is [Fork _] *)
+        destruct Hstep as (v1 & v2 & k & ->).
+        simpl try2. construct_wp_nonret.
+        remember (v1, v2) as p.
+        destruct_thread_step.
+        eassert (thread_step (σ', Stop CFork (v1, v2) k, dom π) _).
+        { eapply ForkS. eassumption. }
+        spec_step.
+        ewp_mask_elim. iMod "Hwp" as "(Hwp & $)".
+        iModIntro.
+        iApply ("IH" with "Hwp"). }
+      (* Get more information out of [e2]; *)
+      construct_wp_nonret.
+      pose proof (can_step_try2 _ _ f Hstep) as Hstep2.
+      pose proof (invert_can_step_thread_step _ _ _ _ _ _ Hstep0 Hstep2) as (_ & ->).
+      eapply invert_thread_step_try2 in Hstep0; last assumption.
+      destruct Hstep0 as (?&->&Hstep0).
+      (* Can use information from above to get [wp] about stepped computation *)
+      spec_step.
+      ewp_mask_elim. iDestruct "Hwp" as ">(Hwp & $)"; iFrame.
+      iModIntro.
+      (* Apply induction hypothesis  *)
+      by iApply ("IH" with "Hwp"). }
+    (* Case: [WPJoin] *)
+    { simpl. ewp_unfold_all.
+      intro_state. spec_state. iMod "Hwp".
+      destruct (π !! x); last done.
+      iDestruct "Hwp" as "(%φ' & $ & Hwp)".
+      iIntros "!> !> %o Ho". iSpecialize ("Hwp" with "Ho").
+      ewp_mask_elim.
+      iMod "Hwp" as "[Hwp $]".
+      iModIntro.
+      iApply ("IH" with "Hwp"). }
+  Qed.
+
+  Lemma ewp_try {B X'} m (f : A -> micro B X') (h : X -> micro B X') Φ :
+    ewp_def E m Ψ
+      (λ o, match o with
+            | O2Ret v => ewp_def E (f v) Ψ Φ
+            | O2Throw e => ewp_def E (h e) Ψ Φ
+            end) -∗
+    ewp_def E (try m f h) Ψ Φ.
+  Proof.
+    iIntros "Hwp".
+    iApply ewp_try2.
+    iApply (ewp_mono with "Hwp").
+    iIntros ([|]) "Hwp"; by cbn.
+  Qed.
+
+  (** *Bind rule *)
+  Lemma ewp_bind {B} m (k : _ -> micro B X) Φ :
+    ewp_def E m  Ψ
+      (λ o, match o with
+            | O2Ret v => ewp_def E (k v) Ψ Φ
+            | O2Throw e => Φ (O2Throw e)
+            end) -∗
+    ewp_def E (bind m k) Ψ Φ.
+  Proof.
+    iIntros "Hwp". rewrite bind_as_try. iApply ewp_try.
+    iApply (ewp_mono with "[$]").
+    iIntros ([v|e]).
+    - iIntros "$".
+    - iIntros "Hexn".
+      iApply (ewp_throw with "Hexn").
+  Qed.
+
+  (* Par combinator *)
+
+  Lemma ewp_Par {A1 A2 X'} (m1 : micro A1 X') (m2 : micro A2 X')
+    (k: outcome2 (A1 * A2) X' → micro A X) Φ1 Φ2 :
+    ewp_def E m1 Ψ Φ1 -∗
+    ewp_def E m2 Ψ Φ2 -∗
+    (∀ e, Φ1 (O2Throw e) -∗ ▷ ewp_def E (k (O2Throw e)) Ψ Q) ∧
+    (∀ e, Φ2 (O2Throw e) -∗ ▷ ewp_def E (k (O2Throw e)) Ψ Q) ∧
+    (∀ v1 v2,
+       Φ1 (O2Ret v1) -∗ Φ2 (O2Ret v2) -∗
+       ▷ ewp_def E (k (O2Ret (v1, v2))) Ψ Q) -∗
+    ewp_def E (Par m1 m2 k) Ψ Q.
+  Proof.
+    iIntros "H1 H2 Hjoin".
+    (* We proceed by Löb-induction after generalizing [m1] [m2] and [k]. *)
+    iLöb as "IH" forall (m1 m2).
+
+    ewp_unfold_head.
+    intro_state.
+
+    ewp_mask_intro "Hmod".
+    construct_wp_nonret; destruct_thread_step; cbn; iMod "Hmod" as "_"; cbn; rename π into π'.
+
+    { (* Case: [StepParRetRet].. *)
+      ewp_invert; iRename "HΦ" into "HΦ2"; ewp_invert; iFrame.
+      iMod "HΦ". iMod "HΦ2".
+      iSpecialize ("Hjoin" with "HΦ HΦ2").
+      ewp_mask_intro "Hmod"; ewp_mask_elim.
+      iApply "Hjoin". }
+
+    (* In the four following cases, one of the branches of the [Par] is either a
+     [crash] or [throw _].
+
+     We invert the cases where there are premises of the form [WP crash _] or
+     [WP (throw _) _] *)
+     1-4: ewp_invert; try done.
+
+    (* [StepParThrowLeft/Right] *)
+    { iMod "HΦ".
+      iDestruct "Hjoin" as "[Hexn1 _]".
+      iSpecialize ("Hexn1" with "[$]").
+      ewp_mask_intro "Hmod"; ewp_mask_elim; iFrame. }
+    { iMod "HΦ".
+      iDestruct "Hjoin" as "[_ [Hexn2 _]]".
+      iSpecialize ("Hexn2" with "[$]").
+      ewp_mask_intro "Hmod"; ewp_mask_elim; iFrame. }
+
+    { (* [StepThroughParLeft]. *)
+      destruct_code.
+      - (* [ParPerformLeft] *)
+        ewp_mask_intro "Hmod"; ewp_mask_elim; iFrame.
+        ewp_unfold (Stop CPerf x k0).
+        ewp_unfold_head.
+        iMod "H1"; iModIntro.
+
+        iApply (monotonic_prot with "[H2 Hjoin] H1").
+        iIntros (?) "Hk".
+        iNext.
+        iApply ("IH" with "Hk H2 Hjoin").
+
+      - (* Step then [ForkS]. *)
+        ewp_mask_intro "Hmod"; ewp_mask_elim; iFrame.
+        destruct x.
+        rewrite (ewp_unfold (Stop CFork (v, v0) _)) /ewp_pre /=.
+        ewp_unfold_head. intro_state. spec_state. iModIntro.
+        construct_wp_nonret. destruct_thread_step.
+        epose proof (ForkS _ _ _ _ _ _ H0).
+        iSpecialize ("H1" $! _ _ _ H1).
+        ewp_mask_elim. iMod "H1" as "(H1 & $)".
+        iApply ("IH" with "H1 H2 Hjoin").
+
+      - (* Step then [JoinS]. *)
+        ewp_mask_intro "Hmod"; ewp_mask_elim; iFrame.
+        rewrite (ewp_unfold (Stop CJoin x _)) /ewp_pre /=.
+        ewp_unfold_head. intro_state. spec_state. iMod "H1".
+        destruct (π !! x); last done.
+        iDestruct "H1" as "(%φ' & $ & H1)".
+        iIntros "!> !> %o Ho". iSpecialize ("H1" with "Ho").
+        ewp_mask_elim. iMod "H1" as "(H1 & $)".
+        iApply ("IH" with "H1 H2 Hjoin"). }
+
+    { (* [StepThroughParRight]. *)
+      destruct_code.
+
+      - (* [StepParPerformRight] *)
+        ewp_mask_intro "Hmod"; ewp_mask_elim; iFrame.
+        ewp_unfold (Stop CPerf x k0).
+        ewp_unfold_head.
+        iMod "H2"; iModIntro.
+        iApply (monotonic_prot with "[H1 Hjoin] H2").
+        iIntros (?) "H2".
+        iNext.
+        iApply ("IH" with "H1 H2 Hjoin").
+
+      - (* [StepParForkRight] *)
+        ewp_mask_intro "Hmod"; ewp_mask_elim; iFrame.
+        destruct x.
+        rewrite (ewp_unfold (Stop CFork (v, v0) _)) /ewp_pre /=.
+        ewp_unfold_head. intro_state. spec_state. iModIntro.
+        construct_wp_nonret. destruct_thread_step.
+        epose proof (ForkS _ _ _ _ _ _ H0).
+        iSpecialize ("H2" $! _ _ _ H1).
+        ewp_mask_elim. iMod "H2" as "(H2 & $)".
+        iApply ("IH" with "H1 H2 Hjoin").
+
+      - (* [StepParJoinRight] *)
+        ewp_mask_intro "Hmod"; ewp_mask_elim; iFrame.
+        rewrite (ewp_unfold (Stop CJoin x _)) /ewp_pre /=.
+        ewp_unfold_head. intro_state. spec_state. iMod "H2".
+        destruct (π !! x); last done.
+        iDestruct "H2" as "(%φ' & $ & H2)".
+        iIntros "!> !> %o Ho". iSpecialize ("H2" with "Ho").
+        ewp_mask_elim. iMod "H2" as "(H2 & $)".
+        iApply ("IH" with "H1 H2 Hjoin"). }
+
+    { (* [ParLeft] *)
+      eapply BaseS in H as Hstep.
+      iCombine "Hsi Hti" as "Hsi".
+      iPoseProof (ewp_step _ _ _ Hstep with "Hsi H1") as ">H1".
+      iMod "H1". ewp_mask_elim. iMod "H1" as "(H1 & $)".
+      iApply ("IH" with "H1 H2 Hjoin"). }
+
+    { (* [ParRight] *)
+      eapply BaseS in H as Hstep.
+      iCombine "Hsi Hti" as "Hsi".
+      iPoseProof (ewp_step _ _ _ Hstep with "Hsi H2") as ">H2".
+      iMod "H2". ewp_mask_elim. iMod "H2" as "(H2 & $)".
+      iApply ("IH" with "H1 H2 Hjoin"). }
+  Qed.
+
+End ewp_rules.
